Exclusivity.v
@@ -14,34 +14,36 @@ Definition init_cr_exclusivity (ths : threads) := forall ad tid1 tid2,
 
 (* theorems ---------------------------------------------------------------- *)
 
-Theorem oneinit_from_insert : forall m ths tid t ad' t',
+Theorem oneinit_from_init : forall m ths tid t ad' t',
   forall_threads ths (valid_term m) ->
   forall_threads ths (consistent_term m) ->
   unique_initializers m ths ->
   (* --- *)
-  ths[tid] --[e_insert ad' t']--> t ->
+  ths[tid] --[e_init ad' t']--> t ->
   one_init ad' ths[tid].
 Proof.
   intros * ? ? Hui **.
-  assert (Had'  : ad' < #m) by eauto using vtm_insert_address.
-  assert (Hnone : m[ad'].t = None) by eauto using insert_then_uninitialized.
+  assert (Had'  : ad' < #m) by eauto using vtm_init_address.
+  assert (Hnone : m[ad'].t = None) by eauto using init_then_uninitialized.
   specialize (Hui ad' Had') as [_ Hui]. specialize (Hui Hnone) as [tid' [? ?]].
   nat_eq_dec tid' tid; trivial.
-  exfalso. eauto using noinit_insert_contradiction.
+  exfalso. eauto using noinit_init_contradiction.
 Qed.
 
 Theorem onecr_from_rel : forall m ths tid t ad',
-  unique_critical_regions m ths ->
+  unique_holding m ths ->
   (* --- *)
   ths[tid] --[e_rel ad']--> t ->
   one_cr ad' ths[tid].
 Proof.
-  intros * Hucr **. specialize (Hucr ad') as [Hfalse Htrue].
+  intros * Huhg **. specialize (Huhg ad') as [Hfalse Htrue].
   destruct (m[ad'].X) eqn:?.
-  - specialize (Htrue eq_refl) as [tid' [? ?]]; clear Hfalse.
+  - specialize (Htrue eq_refl) as [tid' [[? ?] Hnhg]]; clear Hfalse.
     nat_eq_dec tid' tid; trivial.
+    specialize (Hnhg tid). spec. destruct Hnhg as [? | [? ?]]; trivial.
     exfalso. eauto using nocr_rel_contradiction.
   - specialize (Hfalse eq_refl); clear Htrue.
+    specialize (Hfalse tid) as [? | [? ?]]; trivial.
     exfalso. eauto using nocr_rel_contradiction.
 Qed.
 
@@ -77,31 +79,28 @@ Proof.
   exfalso; eauto using onecr_inheritance_alloc, nocr_onecr_contradiction.
 Qed.
 
-Lemma ice_preservation_insert : forall m ths tid t ad' t',
+Lemma ice_preservation_init : forall m ths tid t ad' t',
   forall_threads ths (valid_term m) ->
   forall_threads ths (consistent_term m) ->
   unique_initializers m ths ->
-  unique_critical_regions m ths ->
+  unique_holding m ths ->
   (* --- *)
   init_cr_exclusivity ths ->
-  ths[tid] --[e_insert ad' t']--> t ->
+  ths[tid] --[e_init ad' t']--> t ->
   init_cr_exclusivity ths[tid <- t].
 Proof.
   intros until 4. intros Hice ? ad tid1 tid2.
   destruct (Hice ad tid1 tid2) as [? ?].
   split; intros; repeat omicron; auto; nat_eq_dec ad' ad;
-  eauto using nocr_preservation_insert, oneinit_inheritance_insert;
-  eauto using noinit_preservation_insert, onecr_inheritance_insert;
+  eauto using nocr_preservation_init, oneinit_inheritance_init;
+  eauto using noinit_preservation_init, onecr_inheritance_init;
   exfalso.
-  - assert (one_init ad ths[tid2]) by eauto using oneinit_from_insert.
+  - assert (one_init ad ths[tid2]) by eauto using oneinit_from_init.
     assert (no_init ad t) by eauto using oneinit_to_noinit.
     eauto using noinit_oneinit_contradiction.
-  - assert (one_init ad ths[tid1]) by eauto using oneinit_from_insert.
+  - assert (one_init ad ths[tid1]) by eauto using oneinit_from_init.
     assert (no_init ad t) by eauto using oneinit_to_noinit.
     eauto using noinit_oneinit_contradiction.
-  - assert (one_cr ad ths[tid2]) by eauto using onecr_inheritance_insert.
-    eauto using noinit_insert_contradiction.
-  - eauto using noinit_insert_contradiction.
 Qed.
 
 Lemma ice_preservation_read : forall m ths tid t ad' t',
@@ -187,7 +186,7 @@ Proof.
 Qed.
 
 Lemma ice_preservation_rel : forall m ths tid t ad,
-  unique_critical_regions m ths ->
+  unique_holding m ths ->
   (* --- *)
   init_cr_exclusivity ths ->
   ths[tid] --[e_rel ad]--> t ->
@@ -199,19 +198,40 @@ Proof.
   split; intros; repeat omicron; auto; nat_eq_dec ad' ad;
   eauto using nocr_preservation_rel, oneinit_inheritance_rel;
   eauto using noinit_preservation_rel, onecr_inheritance_rel;
-  eauto using onecr_from_rel;
-  exfalso.
-  - eauto using onecr_from_rel, noinit_preservation_rel,
-      noinit_oneinit_contradiction.
-  - eauto using onecr_from_rel, nocr_onecr_contradiction.
-  - eauto using onecr_from_rel, onecr_to_nocr, nocr_onecr_contradiction.
+  eauto using onecr_from_rel, noinit_preservation_rel.
+Qed.
+
+Lemma ice_preservation_wacq : forall ths tid t ad,
+  init_cr_exclusivity ths ->
+  ths[tid] --[e_wacq ad]--> t ->
+  init_cr_exclusivity ths[tid <- t].
+Proof.
+  intros *. rename ad into ad'.
+  intros Hice ? ad tid1 tid2.
+  destruct (Hice ad tid1 tid2) as [? ?].
+  split; intros; repeat omicron; auto; nat_eq_dec ad' ad;
+  eauto using nocr_preservation_wacq, oneinit_inheritance_wacq;
+  eauto using noinit_preservation_wacq, onecr_inheritance_wacq.
+Qed.
+
+Lemma ice_preservation_wrel : forall ths tid t ad,
+  init_cr_exclusivity ths ->
+  ths[tid] --[e_wrel ad]--> t ->
+  init_cr_exclusivity ths[tid <- t].
+Proof.
+  intros *. rename ad into ad'.
+  intros Hice ? ad tid1 tid2.
+  destruct (Hice ad tid1 tid2) as [? ?].
+  split; intros; repeat omicron; auto; nat_eq_dec ad' ad;
+  eauto using nocr_preservation_wrel, oneinit_inheritance_wrel;
+  eauto using noinit_preservation_wrel, onecr_inheritance_wrel.
 Qed.
 
 Lemma ice_preservation_spawn : forall m ths tid t te,
   forall_threads ths (valid_term m) ->
   (* --- *)
   init_cr_exclusivity ths ->
-  ths[tid] --[e_spawn (#ths) te]--> t ->
+  ths[tid] --[e_spawn te]--> t ->
   init_cr_exclusivity (ths[tid <- t] +++ te).
 Proof.
   intros until 1.
@@ -233,7 +253,7 @@ Theorem ice_preservation_cstep : forall m1 m2 ths1 ths2 tid e,
   forall_program m1 ths1 (consistent_term m1) ->
   no_uninitialized_references m1 ths1         ->
   unique_initializers m1 ths1                 ->
-  unique_critical_regions m1 ths1             ->
+  unique_holding m1 ths1                      ->
   (* --- *)
   init_cr_exclusivity ths1                    ->
   m1 \ ths1 ~~[tid, e]~~> m2 \ ths2           ->
@@ -242,27 +262,14 @@ Proof.
   intros * ? [? ?] [? ?] **. invc_cstep; try invc_mstep.
   - eauto using ice_preservation_none.
   - eauto using ice_preservation_alloc.
-  - eauto using ice_preservation_insert.
+  - eauto using ice_preservation_init.
   - eauto 8 using noinits_from_value, nocrs_from_value, ice_preservation_read.
   - eauto using ice_preservation_write.
   - eauto 8 using noinits_from_value, nocrs_from_value, ice_preservation_acq.
   - eauto using ice_preservation_rel.
+  - eauto using ice_preservation_wacq.
+  - eauto using ice_preservation_wrel.
   - eauto using ice_preservation_spawn.
-Qed.
-
-Theorem ice_preservation_rstep : forall m1 m2 ths1 ths2 tid e,
-  forall_memory  m1      value                ->
-  forall_program m1 ths1 (valid_term m1)      ->
-  forall_program m1 ths1 (consistent_term m1) ->
-  no_uninitialized_references m1 ths1         ->
-  unique_initializers m1 ths1                 ->
-  unique_critical_regions m1 ths1             ->
-  (* --- *)
-  init_cr_exclusivity ths1                    ->
-  m1 \ ths1 ~~~[tid, e]~~> m2 \ ths2          ->
-  init_cr_exclusivity ths2.
-Proof.
-  intros. invc_rstep; eauto using ice_preservation_cstep.
 Qed.
 
 Theorem ice_preservation_base : forall t,
@@ -289,7 +296,7 @@ Definition term_init_cr_exc (t : tm) := forall ad,
 Local Ltac solve_inv_tice :=
   intros * H; repeat match goal with |- _ /\ _ => split end; intros ad';
   specialize (H ad') as [[? | ?] [[? | ?] [? ?]]]; repeat split; repeat spec;
-  try inv_oneinit; try inv_onecr; try inv_nocr; try inv_noinit; auto; intros ?;
+  try inv_oneinit; try inv_onecr; try inv_nocr; try inv_noinit; auto; intro;
   exfalso; eauto using noinit_oneinit_contradiction, nocr_onecr_contradiction. 
 
 Local Lemma inv_tice_plus : forall t1 t2,
@@ -304,32 +311,17 @@ Proof. solve_inv_tice. Qed.
 
 Local Lemma inv_tice_seq : forall t1 t2,
   term_init_cr_exc <{t1; t2}> ->
-  term_init_cr_exc t1 /\ term_init_cr_exc t2.
+  term_init_cr_exc t1.
 Proof. solve_inv_tice. Qed.
 
 Local Lemma inv_tice_if : forall t1 t2 t3,
   term_init_cr_exc <{if t1 then t2 else t3 end}> ->
-  term_init_cr_exc t1 /\ term_init_cr_exc t2 /\ term_init_cr_exc t3.
-Proof. solve_inv_tice. Qed.
-
-Local Lemma inv_tice_while : forall t1 t2,
-  term_init_cr_exc <{while t1 do t2 end}> ->
-  term_init_cr_exc t1 /\ term_init_cr_exc t2.
-Proof. solve_inv_tice. Qed.
-
-Local Lemma inv_tice_fun : forall x Tx t,
-  term_init_cr_exc <{fn x Tx t}> ->
-  term_init_cr_exc t.
+  term_init_cr_exc t1.
 Proof. solve_inv_tice. Qed.
 
 Local Lemma inv_tice_call : forall t1 t2,
   term_init_cr_exc <{call t1 t2}> ->
   term_init_cr_exc t1 /\ term_init_cr_exc t2.
-Proof. solve_inv_tice. Qed.
-
-Local Lemma inv_tice_new : forall t T,
-  term_init_cr_exc <{new t : T}> ->
-  term_init_cr_exc t.
 Proof. solve_inv_tice. Qed.
 
 Local Lemma inv_tice_init : forall ad t T,
@@ -349,7 +341,7 @@ Proof. solve_inv_tice. Qed.
 
 Local Lemma inv_tice_acq : forall t1 x t2,
   term_init_cr_exc <{acq t1 x t2}> ->
-  term_init_cr_exc t1 /\ term_init_cr_exc t2.
+  term_init_cr_exc t1.
 Proof. solve_inv_tice. Qed.
 
 Local Lemma inv_tice_cr : forall ad t,
@@ -357,8 +349,8 @@ Local Lemma inv_tice_cr : forall ad t,
   term_init_cr_exc t.
 Proof. solve_inv_tice. Qed.
 
-Local Lemma inv_tice_spawn : forall t,
-  term_init_cr_exc <{spawn t}> ->
+Local Lemma inv_tice_wait : forall t,
+  term_init_cr_exc <{wait t}> ->
   term_init_cr_exc t.
 Proof. solve_inv_tice. Qed.
 
@@ -370,18 +362,18 @@ Ltac invc_tice :=
   | H : term_init_cr_exc <{_ - _       }> |- _ => eapply inv_tice_monus in H
   | H : term_init_cr_exc <{_; _        }> |- _ => eapply inv_tice_seq   in H
   | H : term_init_cr_exc (tm_if _ _ _  )  |- _ => eapply inv_tice_if    in H
-  | H : term_init_cr_exc (tm_while _ _ )  |- _ => eapply inv_tice_while in H
+  | H : term_init_cr_exc (tm_while _ _ )  |- _ => clear H
   | H : term_init_cr_exc <{var _       }> |- _ => clear H
-  | H : term_init_cr_exc <{fn _ _ _    }> |- _ => eapply inv_tice_fun   in H
+  | H : term_init_cr_exc <{fn _ _ _    }> |- _ => clear H
   | H : term_init_cr_exc <{call _ _    }> |- _ => eapply inv_tice_call  in H
   | H : term_init_cr_exc <{& _ : _     }> |- _ => clear H
-  | H : term_init_cr_exc <{new _ : _   }> |- _ => eapply inv_tice_new   in H
+  | H : term_init_cr_exc <{new _ : _   }> |- _ => clear H
   | H : term_init_cr_exc <{init _ _ : _}> |- _ => eapply inv_tice_init  in H
   | H : term_init_cr_exc <{* _         }> |- _ => eapply inv_tice_load  in H
   | H : term_init_cr_exc <{_ := _      }> |- _ => eapply inv_tice_asg   in H
   | H : term_init_cr_exc <{acq _ _ _   }> |- _ => eapply inv_tice_acq   in H
   | H : term_init_cr_exc <{cr _ _      }> |- _ => eapply inv_tice_cr    in H
-  | H : term_init_cr_exc <{spawn _     }> |- _ => eapply inv_tice_spawn in H
+  | H : term_init_cr_exc <{spawn _     }> |- _ => clear H
   end;
   repeat match goal with
   | H : term_init_cr_exc _ /\ term_init_cr_exc _ |- _ => destruct H
@@ -392,13 +384,14 @@ Ltac invc_tice :=
 Theorem tice_from_ice : forall m ths,
   forall_threads ths (valid_term m) ->
   unique_initializers m ths ->
-  unique_critical_regions m ths ->
+  unique_holding m ths ->
   (* --- *)
   init_cr_exclusivity ths ->
   forall_threads ths term_init_cr_exc.
 Proof.
-  intros * ? Hui Hucr Hice tid ad. specialize (Hice ad tid tid) as [? ?].
-  eauto 6 using noinit_or_oneinit_from_ui, nocr_or_onecr_from_ucr.
+  intros * ? Hui Huhg Hice tid ad. specialize (Hice ad tid tid) as [? ?];
+  repeat split; eauto;
+  eauto 6 using noinit_or_oneinit_from_ui, nocr_or_onecr_from_uhg.
 Qed.
 
 Theorem nocr_from_acq : forall m ths tid t ad' t',
