Holding.v
@@ -1,0 +1,302 @@
+From Elo Require Import Core.
+
+From Elo Require Import NoCR.
+From Elo Require Import NoReacq.
+From Elo Require Import ValidTerm.
+From Elo Require Import ConsistentWaits.
+From Elo Require Import OneCR.
+From Elo Require Import Waiting.
+
+(* ------------------------------------------------------------------------- *)
+(* holding & not-holding                                                     *)
+(* ------------------------------------------------------------------------- *)
+
+Definition holding (ad : addr) (t : tm) :=
+  one_cr ad t /\ no_reacq ad t.
+
+Definition not_holding (ad : addr) (t : tm) :=
+  no_cr ad t \/ (one_cr ad t /\ waiting ad t).
+
+(* lemmas ------------------------------------------------------------------ *)
+
+Corollary hg_contradiction : forall ad t,
+  not_holding ad t ->
+  holding     ad t ->
+  False.
+Proof.
+  intros * [? | [? ?]] [? ?];
+  eauto using nocr_onecr_contradiction, noreacq_wg_contradiction.
+Qed.
+
+Corollary nhg_unit : forall ad,
+  not_holding ad <{unit}>.
+Proof.
+  intros. left. auto using no_cr.
+Qed.
+
+Corollary nhg_from_value : forall m ad t,
+  valid_term m t ->
+  (* --- *)
+  value t ->
+  not_holding ad t.
+Proof.
+  intros. left. eauto using nocr_from_value.
+Qed.
+
+(* preservation (holding) -------------------------------------------------- *)
+
+Local Ltac solve_hg_preservation L1 L2 :=
+  intros; match goal with H : holding _ _ |- _ => destruct H end; split;
+  eauto using nocr_from_value, noreacq_from_value, L1, L2.
+
+Corollary hg_preservation_none : forall ad m t1 t2,
+  valid_term m t1 ->
+  (* --- *)
+  holding ad t1 ->
+  t1 --[e_none]--> t2 ->
+  holding ad t2.
+Proof.
+  solve_hg_preservation
+    onecr_preservation_none
+    noreacq_preservation_none.
+Qed.
+
+Corollary hg_preservation_alloc : forall ad t1 t2 ad' T',
+  holding ad t1 ->
+  t1 --[e_alloc ad' T']--> t2 ->
+  holding ad t2.
+Proof.
+  solve_hg_preservation
+    onecr_preservation_alloc
+    noreacq_preservation_alloc.
+Qed.
+
+Corollary hg_preservation_init : forall ad m t1 t2 ad' t',
+  valid_term m t1 ->
+  (* --- *)
+  holding ad t1 ->
+  t1 --[e_init ad' t']--> t2 ->
+  holding ad t2.
+Proof.
+  solve_hg_preservation
+    onecr_preservation_init
+    noreacq_preservation_init.
+Qed.
+
+Corollary hg_preservation_read : forall ad m t1 t2 ad' t',
+  valid_term m t' ->
+  value t'        ->
+  (* --- *)
+  holding ad t1 ->
+  t1 --[e_read ad' t']--> t2 ->
+  holding ad t2.
+Proof.
+  solve_hg_preservation
+    onecr_preservation_read
+    noreacq_preservation_read.
+Qed.
+
+Corollary hg_preservation_write : forall ad m t1 t2 ad' t',
+  valid_term m t1 ->
+  (* --- *)
+  holding ad t1 ->
+  t1 --[e_write ad' t']--> t2 ->
+  holding ad t2.
+Proof.
+  solve_hg_preservation
+    onecr_preservation_write
+    noreacq_preservation_write.
+Qed.
+
+Corollary hg_preservation_acq : forall ad m t1 t2 ad' t',
+  valid_term m t' ->
+  value t'        ->
+  (* --- *)
+  ad <> ad' ->
+  holding ad t1 ->
+  t1 --[e_acq ad' t']--> t2 ->
+  holding ad t2.
+Proof.
+  solve_hg_preservation
+    onecr_preservation_acq
+    noreacq_preservation_acq.
+Qed.
+
+Corollary hg_preservation_rel : forall ad t1 t2 ad',
+  ad <> ad' ->
+  holding ad t1 ->
+  t1 --[e_rel ad']--> t2 ->
+  holding ad t2.
+Proof.
+  solve_hg_preservation
+    onecr_preservation_rel
+    noreacq_preservation_rel.
+Qed.
+
+Corollary hg_preservation_wacq : forall ad t1 t2 ad',
+  holding ad t1 ->
+  t1 --[e_wacq ad']--> t2 ->
+  holding ad t2.
+Proof.
+  solve_hg_preservation
+    onecr_preservation_wacq
+    noreacq_preservation_wacq.
+Qed.
+
+Corollary hg_preservation_wrel : forall ad t1 t2 ad',
+  ad <> ad' ->
+  holding ad t1 ->
+  t1 --[e_wrel ad']--> t2 ->
+  holding ad t2.
+Proof.
+  solve_hg_preservation
+    onecr_preservation_wrel
+    noreacq_preservation_wrel.
+Qed.
+
+Corollary hg_preservation_spawn : forall ad m t1 t2 t',
+  valid_term m t1 ->
+  (* --- *)
+  holding ad t1 ->
+  t1 --[e_spawn t']--> t2 ->
+  holding ad t2.
+Proof.
+  solve_hg_preservation
+    onecr_preservation_spawn
+    noreacq_preservation_spawn.
+Qed.
+
+(* preservation  (nholding) --------------------------------------------------- *)
+
+Local Ltac solve_nhg_preservation L1 L2 L3 :=
+  intros;
+  match goal with H : not_holding _ _ |- _ => destruct H as [? | [? ?]] end;
+  solve [ left; eauto using nocr_from_value, L1
+        | right; split; eauto using nocr_from_value, noreacq_from_value, L2, L3
+        ].
+
+Corollary nhg_preservation_none : forall ad m t1 t2,
+  valid_term m t1 ->
+  (* --- *)
+  not_holding ad t1 ->
+  t1 --[e_none]--> t2 ->
+  not_holding ad t2.
+Proof.
+  solve_nhg_preservation
+    nocr_preservation_none
+    onecr_preservation_none wg_preservation_none.
+Qed.
+
+Corollary nhg_preservation_alloc : forall ad t1 t2 ad' T',
+  not_holding ad t1 ->
+  t1 --[e_alloc ad' T']--> t2 ->
+  not_holding ad t2.
+Proof.
+  solve_nhg_preservation
+    nocr_preservation_alloc
+    onecr_preservation_alloc wg_preservation_alloc.
+Qed.
+
+Corollary nhg_preservation_init : forall ad m t1 t2 ad' t',
+  valid_term m t1 ->
+  (* --- *)
+  not_holding ad t1 ->
+  t1 --[e_init ad' t']--> t2 ->
+  not_holding ad t2.
+Proof.
+  solve_nhg_preservation
+    nocr_preservation_init
+    onecr_preservation_init wg_preservation_init.
+Qed.
+
+Corollary nhg_preservation_read : forall ad m t1 t2 ad' t',
+  valid_term m t' ->
+  value t'        ->
+  (* --- *)
+  not_holding ad t1 ->
+  t1 --[e_read ad' t']--> t2 ->
+  not_holding ad t2.
+Proof.
+  solve_nhg_preservation
+    nocr_preservation_read
+    onecr_preservation_read wg_preservation_read.
+Qed.
+
+Corollary nhg_preservation_write : forall ad m t1 t2 ad' t',
+  valid_term m t1 ->
+  (* --- *)
+  not_holding ad t1 ->
+  t1 --[e_write ad' t']--> t2 ->
+  not_holding ad t2.
+Proof.
+  solve_nhg_preservation
+    nocr_preservation_write
+    onecr_preservation_write wg_preservation_write.
+Qed.
+
+Corollary nhg_preservation_acq : forall ad m t1 t2 ad' t',
+  valid_term m t' ->
+  value t'        ->
+  (* --- *)
+  ad <> ad' ->
+  not_holding ad t1 ->
+  t1 --[e_acq ad' t']--> t2 ->
+  not_holding ad t2.
+Proof.
+  solve_nhg_preservation
+    nocr_preservation_acq
+    onecr_preservation_acq wg_preservation_acq.
+Qed.
+
+Corollary nhg_preservation_rel : forall ad t1 t2 ad',
+  ad <> ad' ->
+  not_holding ad t1 ->
+  t1 --[e_rel ad']--> t2 ->
+  not_holding ad t2.
+Proof.
+  solve_nhg_preservation
+    nocr_preservation_rel
+    onecr_preservation_rel wg_preservation_rel.
+Qed.
+
+Corollary nhg_preservation_wacq : forall ad t1 t2 ad',
+  ad <> ad' ->
+  not_holding ad t1 ->
+  t1 --[e_wacq ad']--> t2 ->
+  not_holding ad t2.
+Proof.
+  solve_nhg_preservation
+    nocr_preservation_wacq
+    onecr_preservation_wacq wg_preservation_wacq.
+Qed.
+
+Corollary nhg_preservation_wrel : forall m ad t1 t2 ad',
+  valid_term m t1             ->
+  consistent_waits WR_none t1 ->
+  (* --- *)
+  not_holding ad t1 ->
+  t1 --[e_wrel ad']--> t2 ->
+  not_holding ad t2.
+Proof.
+  intros * ? ? H **.
+  assert (ad <> ad'). {
+    intro. subst. destruct H as [? | [? ?]];
+    eauto using nocr_wrel_contradiction, wg_effect_contradiction.
+  }
+  solve_nhg_preservation
+    nocr_preservation_wrel
+    onecr_preservation_wrel wg_preservation_wrel.
+Qed.
+
+Corollary nhg_preservation_spawn : forall ad m t1 t2 t',
+  valid_term m t1 ->
+  (* --- *)
+  not_holding ad t1 ->
+  t1 --[e_spawn t']--> t2 ->
+  not_holding ad t2.
+Proof.
+  solve_nhg_preservation
+    nocr_preservation_spawn
+    onecr_preservation_spawn wg_preservation_spawn.
+Qed.
+
