Soundness.v
@@ -21,6 +21,30 @@ Proof.
 Qed.
 
 (* TODO: rename *)
+Lemma aux_inc1'' : forall Gamma k T T1 T2,
+  k <> SELF ->
+  (safe Gamma)[SELF <== T][k <== T2]
+    includes
+  (safe Gamma[k <== T1])[SELF <== T][k <== T2].
+Proof.
+  intros * ? k' T' H.
+  eapply MapInc.update_permutation; auto.
+  eapply MapInc.update_permutation in H; auto.
+  eapply MapInc.update_inclusion; eauto.
+  eauto using aux_inc1.
+Qed.
+
+(*
+i <> SELF
+
+1: ((safe Gamma) [SELF <== ` x& Tx0 `]) [i <== Tx']
+
+2: ((safe Gamma [i <== Tx]) [SELF <== `x&Tx'`]) [i <== Tx']
+
+    1 includes 2
+*)
+
+(* TODO: rename *)
 Lemma aux_inc2 : forall Gamma k k' T T',
   k <> k' ->
   (safe Gamma)[k' <== T'][k <== T] includes (safe Gamma[k <== T])[k' <== T'].
@@ -30,32 +54,50 @@ Proof.
 Qed.
 
 Lemma typeof_subst : forall t tx T Tx Gamma x,
+  keywords t ->
   Gamma[x <== Tx] |-- t is T ->
   empty |-- tx is Tx ->
   Gamma |-- <{[x := tx] t}> is T.
 Proof.
-  intros ?. induction t; intros * Htype ?; invc_typeof; eauto using type_of;
-  simpl; try destruct _str_eq_dec; subst;
+  intros ?. induction t; intros * Htype ?;
+  invc_kw; invc_typeof; eauto using type_of;
+  simpl; repeat destruct _str_eq_dec; subst;
   eauto using type_of, context_weakening_empty, context_weakening,
     update_safe_includes_safe_update,
     MapInc.update_overwrite, MapInc.update_permutation;
-  try match goal with | H : _[_ <== _] _ = _ |- _ => rename H into Hty end.
+  try match goal with | H : _[_ <== _] _ = _ |- _ => rename H into Hty end;
+  eauto 9 using context_weakening,
+    MapInc.update_permutation, MapInc.update_inclusion,
+    aux_inc1, aux_inc2, type_of.
   - rewrite lookup_update_eq in Hty.
     invc Hty. eauto using context_weakening_empty.
   - rewrite lookup_update_neq in Hty; eauto using type_of.
-  - eauto using aux_inc1, context_weakening, type_of.
-  - eauto 6 using aux_inc2, context_weakening, type_of.
+Qed.
+
+Corollary typeof_subst_self : forall x tx t T Tx ad,
+  keywords t  ->
+  keywords tx ->
+  x <> SELF ->
+  empty |-- tx is Tx ->
+  (safe empty)[SELF <== `x&Tx`][x <== Tx] |-- t is T ->
+  empty |-- <{[SELF := (&ad : x&Tx)][x := tx] t}> is T.
+Proof.
+  intros.
+  eapply typeof_subst; eauto using kw_subst, type_of.
+  eauto using typeof_subst, context_weakening, MapInc.update_permutation.
 Qed.
 
 (* ------------------------------------------------------------------------- *)
 
 Local Ltac solve_typeof_preservation T :=
   intros; gendep T; ind_tstep; intros;
-  repeat invc_ctm; repeat invc_typeof;
-  try invc_eq; eauto using typeof_subst, type_of.
+  repeat invc_kw; repeat invc_ctm; repeat invc_typeof;
+  try invc_eq; eauto using typeof_subst, typeof_subst_self, type_of.
 
 Lemma typeof_preservation_none : forall T t1 t2,
-  empty |-- t1 is T ->
+  keywords t1 ->
+  (* --- *)
+  empty |-- t1 is T   ->
   t1 --[e_none]--> t2 ->
   empty |-- t2 is T.
 Proof. solve_typeof_preservation T. Qed.
@@ -66,9 +108,9 @@ Lemma typeof_preservation_alloc : forall T t1 t2 ad' T',
   empty |-- t2 is T.
 Proof. solve_typeof_preservation T. Qed.
 
-Lemma typeof_preservation_insert : forall T t1 t2 ad' t',
+Lemma typeof_preservation_init : forall T t1 t2 ad' t',
   empty |-- t1 is T ->
-  t1 --[e_insert ad' t']--> t2 ->
+  t1 --[e_init ad' t']--> t2 ->
   empty |-- t2 is T.
 Proof. solve_typeof_preservation T. Qed.
 
@@ -88,6 +130,8 @@ Lemma typeof_preservation_write : forall T t1 t2 ad' t',
 Proof. solve_typeof_preservation T. Qed.
 
 Lemma typeof_preservation_acq : forall T m t1 t2 ad' t',
+  keywords t1          ->
+  keywords t'          ->
   consistent_term m t1 ->
   (* --- *)
   m[ad'].t = Some t' ->
@@ -102,22 +146,36 @@ Lemma typeof_preservation_rel : forall T t1 t2 ad,
   empty |-- t2 is T.
 Proof. solve_typeof_preservation T. Qed.
 
-Lemma typeof_preservation_spawn : forall T t1 t2 tid t,
+Lemma typeof_preservation_wacq : forall T t1 t2 ad',
   empty |-- t1 is T ->
-  t1 --[e_spawn tid t]--> t2 ->
+  t1 --[e_wacq ad']--> t2 ->
   empty |-- t2 is T.
 Proof. solve_typeof_preservation T. Qed.
 
-Lemma typeof_preservation_spawned : forall t1 t2 tid t T1,
+Lemma typeof_preservation_wrel : forall T t1 t2 ad',
+  empty |-- t1 is T ->
+  t1 --[e_wrel ad']--> t2 ->
+  empty |-- t2 is T.
+Proof. solve_typeof_preservation T. Qed.
+
+Lemma typeof_preservation_spawn : forall T t1 t2 t,
+  empty |-- t1 is T ->
+  t1 --[e_spawn t]--> t2 ->
+  empty |-- t2 is T.
+Proof. solve_typeof_preservation T. Qed.
+
+Lemma typeof_preservation_spawned : forall t1 t2 t T1,
   empty |-- t1 is T1 ->
-  t1 --[e_spawn tid t]--> t2 ->
+  t1 --[e_spawn t]--> t2 ->
   exists T, empty |-- t is T.
 Proof.
   intros. gendep T1. ind_tstep; intros; invc_typeof; eauto.
 Qed.
 
 Local Lemma typeof_preservation_mstep : forall m1 m2 t1 t2 e T,
-  consistent_term m1 t1 ->
+  forall_memory m1 keywords ->
+  keywords t1               ->
+  consistent_term m1 t1     ->
   (* --- *)
   empty |-- t1 is T ->
   m1 \ t1 ==[e]==> m2 \ t2 ->
@@ -126,11 +184,13 @@ Proof.
   intros. invc_mstep.
   - eauto using typeof_preservation_none.
   - eauto using typeof_preservation_alloc.
-  - eauto using typeof_preservation_insert.
+  - eauto using typeof_preservation_init.
   - eauto using typeof_preservation_read.
   - eauto using typeof_preservation_write.
   - eauto using typeof_preservation_acq.
   - eauto using typeof_preservation_rel.
+  - eauto using typeof_preservation_wacq.
+  - eauto using typeof_preservation_wrel.
 Qed.
 
 Local Lemma typeof_preservation_mem_mstep : forall m1 m2 t1 t2 t1' t2' e ad T,
@@ -147,7 +207,7 @@ Proof.
   assert (ad' < #m1) by (lt_eq_gt (#m1) ad'; sigma; upsilon; auto).
   invc_mstep; try invc_eq; trivial;
   sigma; try omicron; repeat invc_eq; trivial; upsilon.
-  + assert (m1[ad'].t = None) by eauto using insert_then_uninitialized. invc_eq.
+  + assert (m1[ad'].t = None) by eauto using init_then_uninitialized. invc_eq.
   + gendep T'. gendep t1'. ind_tstep; intros;
     repeat invc_typeof; repeat invc_ctm; repeat invc_ctm; eauto.
     invc_eq. apply_deterministic_typing. assumption.
@@ -159,26 +219,28 @@ Definition types_of (ths : threads) (Ts: list ty) :=
 Notation "'|--' ths 'is' Ts" := (types_of ths Ts) (at level 40).
 
 Theorem typeof_preservation : forall m1 m2 ths1 ths2 Ts tid e,
+  forall_memory  m1   keywords             ->
+  forall_threads ths1 keywords             ->
   forall_threads ths1 (consistent_term m1) ->
   (* --- *)
   |-- ths1 is Ts ->
   m1 \ ths1 ~~[tid, e]~~> m2 \ ths2 ->
   (|-- ths2 is Ts \/ exists T, |-- ths2 is (Ts +++ T)).
 Proof.
-  intros * ? [Heq ?] **. inv_cstep.
-  - left. split; sigma; trivial.
-    intros ?. omicron; eauto using typeof_preservation_mstep.
-  - right.
-    assert (exists T, empty |-- te is T) as [? ?]
-        by eauto using typeof_preservation_spawned.
-    eexists. split; sigma; eauto.
-    intros ?. omicron;
-    repeat match goal with
-    | H : #ths1 < _ |- _ => rewrite Heq in H
-    | H : _ < #ths1 |- _ => rewrite Heq in H
-    | |- context C [ #ths1 ] => rewrite Heq 
-    end;
-    sigma; eauto using typeof_preservation_spawn, type_of.
+  intros * ? ? ? [Heq ?] **. inv_cstep;
+  try solve [left; split; sigma; trivial;
+             intros ?; omicron; eauto using typeof_preservation_mstep].
+  right.
+  assert (exists T, empty |-- t' is T) as [? ?]
+      by eauto using typeof_preservation_spawned.
+  eexists. split; sigma; eauto.
+  intros ?. omicron;
+  repeat match goal with
+  | H : #ths1 < _ |- _ => rewrite Heq in H
+  | H : _ < #ths1 |- _ => rewrite Heq in H
+  | |- context C [ #ths1 ] => rewrite Heq 
+  end;
+  sigma; eauto using typeof_preservation_spawn, type_of.
 Qed.
 
 Lemma forall_array_inversion {A} {d} : forall (P : A -> Prop) x xs,
@@ -213,13 +275,15 @@ Proof.
 Qed.
 
 Lemma wtt_preservation_threads : forall m1 m2 ths1 ths2 tid e,
+  forall_memory  m1   keywords             ->
+  forall_threads ths1 keywords             ->
   forall_threads ths1 (consistent_term m1) ->
   (* --- *)
   forall_threads ths1 well_typed_term ->
   m1 \ ths1 ~~[tid, e]~~> m2 \ ths2 ->
   forall_threads ths2 well_typed_term.
 Proof.
-  intros * ? Hwtt **.
+  intros * ? ? ? Hwtt **.
   eapply wtt_to_typesof in Hwtt as [Ts ?].
   assert (|-- ths2 is Ts \/ exists T, |-- ths2 is (Ts +++ T))
     as [[? ?] | [? [? ?]]] by eauto using typeof_preservation;
@@ -233,36 +297,21 @@ Lemma wtt_preservation_memory : forall m1 m2 ths1 ths2 tid e,
   m1 \ ths1 ~~[tid, e]~~> m2 \ ths2 ->
   forall_memory m2 well_typed_term.
 Proof.
-  intros. invc_cstep; trivial. invc_mstep; trivial;
-  intros ? ? ?; upsilon; eauto using wtt_insert_term, wtt_write_term.
+  intros. invc_cstep; try invc_mstep; trivial;
+  intros ? ? ?; omicron; upsilon; auto;
+  eauto using wtt_init_term, wtt_write_term.
 Qed.
 
 Theorem wtt_preservation_cstep : forall m1 m2 ths1 ths2 tid e,
+  forall_program m1 ths1 keywords             ->
   forall_program m1 ths1 (consistent_term m1) ->
   (* --- *)
   forall_program m1 ths1 well_typed_term ->
-  m1 \ ths1 ~~[tid, e]~~> m2 \ ths2 ->
+  m1 \ ths1 ~~[tid, e]~~> m2 \ ths2      ->
   forall_program m2 ths2 well_typed_term.
 Proof.
-  intros * [_ ?] [? ?] **. split;
+  intros * [? ?] [_ ?] [? ?] **. split;
   eauto using wtt_preservation_memory, wtt_preservation_threads.
-Qed.
-
-Theorem wtt_preservation_rstep : forall m1 m2 ths1 ths2 tid e,
-  forall_program m1 ths1 (consistent_term m1) ->
-  (* --- *)
-  forall_program m1 ths1 well_typed_term ->
-  m1 \ ths1 ~~~[tid, e]~~> m2 \ ths2 ->
-  forall_program m2 ths2 well_typed_term.
-Proof.
-  intros. invc_rstep; eauto using wtt_preservation_cstep.
-  match goal with _ : _ \ _ ~~[_, _]~~> ?m \ ?ths |- _ =>
-    assert (forall_program m ths well_typed_term) as [Hmwtt Hwtt]
-      by eauto using wtt_preservation_cstep
-  end.
-  invc_cstep. invc_mstep.
-  split; intros i; repeat intro; omicron; upsilon; auto;
-  specialize (Hmwtt i); specialize (Hwtt i); sigma; auto.
 Qed.
 
 Theorem wtt_preservation_base : forall t,
@@ -283,154 +332,216 @@ Local Ltac invc_value_typeof :=
   end.
 
 Ltac destructIH IH :=
-  destruct IH as [?Hval | [?t2' [
-    [?m2 [?ad' [?t' ?Hmstep]]] | [[?m2 [?e ?Hmstep]] | [?tid [?t' ?Htstep]]]
+  destruct IH as [?Hval | [?t2'
+    [[?m2 [?ad' [?t' ?Hmstep]]] |
+        [[?m2 [?ad' ?Hmstep]] |
+            [[?m2 [?e ?Hmstep]] |
+                [?t' ?Htstep]]]
   ]]].
 
-Theorem limited_progress : forall m1 t1,
-  valid_term      m1 t1 ->
-  consistent_term m1 t1 ->
+(* Work on this... *)
+Local Ltac solve_intros_He :=
+  match goal with
+  | Hmstep : (forall _ _, _ <> _) -> ?m1 \ ?t2 ==[?e]==> ?m2 \ ?t2'
+  |- (forall _ _, _ <> _) ->
+     ?m1 \ (?c _ ?t2) ==[?e]==> ?m2 \ (?c _ ?t2') =>
+    intros He; specialize (Hmstep He);
+    invc_mstep; eauto using value, tstep, mstep
+  end.
+
+Theorem limited_progress : forall wr m1 t1,
+  wr <> WR_self          ->
+  valid_term m1 t1       ->
+  consistent_waits wr t1 ->
+  consistent_term m1 t1  ->
   (* --- *)
   well_typed_term t1 ->
   (value t1 \/ exists t2,
-  (exists m2 ad t, m1[ad].X = false -> m1 \ t1 ==[e_acq ad t]==> m2 \ t2)   \/
-  (exists m2 e, (forall ad t, e <> e_acq ad t) -> m1 \ t1 ==[e]==> m2 \ t2) \/
-  (exists tid t, t1 --[e_spawn tid t]--> t2)).
+  (exists m2 ad t, m1[ad].X = false -> m1 \ t1 ==[e_acq  ad t ]==> m2 \ t2) \/
+  (exists m2 ad,   m1[ad].X = false -> m1 \ t1 ==[e_wacq ad   ]==> m2 \ t2) \/
+  (exists m2 e, (forall ad t, e <> e_acq ad t /\ forall ad, e <> e_wacq ad) ->
+                                       m1 \ t1 ==[e]==> m2 \ t2) \/
+  (exists t, t1 --[e_spawn t]--> t2)).
 Proof.
-  intros * ? ? [T ?]. remember empty as Gamma.
-  ind_typeof; invc_vtm; invc_ctm; eauto using value; right; repeat spec.
-  - destructIH IHtype_of1.
+  intros * ? ? ? ? [T ?]. remember empty as Gamma. gendep wr.
+  ind_typeof; intros; invc_vtm; invc_cw; invc_ctm;
+  auto; eauto using value; right.
+  - repeat spec. destructIH IHtype_of1.
     + invc_value_typeof. invc_vtm. invc_ctm.
       destructIH IHtype_of2.
       * invc_value_typeof. invc_vtm. invc_ctm.
-        eexists. right. left. eauto using tstep, mstep.
+        eexists. right. right. left. eauto using tstep, mstep.
       * eexists. left. repeat eexists. intros Hfalse.
         specialize (Hmstep Hfalse). invc_mstep. eauto using value, tstep, mstep.
       * eexists. right. left. repeat eexists. intros He.
         specialize (Hmstep He). invc_mstep; eauto using value, tstep, mstep.
-      * eexists. right. right. repeat eexists. eauto using value, tstep.
+      * eexists. right. right. left. repeat eexists. intros He.
+        specialize (Hmstep He). invc_mstep; eauto using value, tstep, mstep.
+      * eexists. right. right. right. repeat eexists. eauto using value, tstep.
     + eexists. left. repeat eexists. intros Hfalse.
       specialize (Hmstep Hfalse). invc_mstep. eauto using tstep, mstep.
     + eexists. right. left. repeat eexists. intros He.
       specialize (Hmstep He). invc_mstep; eauto using tstep, mstep.
+    + eexists. right. right. left. repeat eexists. intros He.
+      specialize (Hmstep He). invc_mstep; eauto using tstep, mstep.
     + eexists. right. right. repeat eexists. eauto using tstep.
-  - destructIH IHtype_of1.
+  - repeat spec. destructIH IHtype_of1.
     + invc_value_typeof. invc_vtm. invc_ctm.
       destructIH IHtype_of2.
       * invc_value_typeof. invc_vtm. invc_ctm.
-        eexists. right. left. eauto using tstep, mstep.
+        eexists. right. right. left. eauto using tstep, mstep.
       * eexists. left. repeat eexists. intros Hfalse.
         specialize (Hmstep Hfalse). invc_mstep. eauto using value, tstep, mstep.
       * eexists. right. left. repeat eexists. intros He.
         specialize (Hmstep He). invc_mstep; eauto using value, tstep, mstep.
-      * eexists. right. right. repeat eexists. eauto using value, tstep.
+      * eexists. right. right. left. repeat eexists. intros He.
+        specialize (Hmstep He). invc_mstep; eauto using value, tstep, mstep.
+      * eexists. right. right. right. repeat eexists. eauto using value, tstep.
     + eexists. left. repeat eexists. intros Hfalse.
       specialize (Hmstep Hfalse). invc_mstep. eauto using tstep, mstep.
     + eexists. right. left. repeat eexists. intros He.
       specialize (Hmstep He). invc_mstep; eauto using tstep, mstep.
+    + eexists. right. right. left. repeat eexists. intros He.
+      specialize (Hmstep He). invc_mstep; eauto using tstep, mstep.
     + eexists. right. right. repeat eexists. eauto using tstep.
-  - destructIH IHtype_of1; eexists.
-    + right. left. eauto using tstep, mstep.
+  - repeat spec. destructIH IHtype_of1; eexists.
+    + right. right. left. eauto using tstep, mstep.
     + left. repeat eexists. intros Hfalse.
       specialize (Hmstep Hfalse). invc_mstep. eauto using tstep, mstep.
     + right. left. repeat eexists. intros He.
       specialize (Hmstep He). invc_mstep; eauto using tstep, mstep.
+    + right. right. left. repeat eexists. intros He.
+      specialize (Hmstep He). invc_mstep; eauto using tstep, mstep.
     + right. right. repeat eexists. eauto using tstep.
-  - destructIH IHtype_of1.
+  - repeat spec. destructIH IHtype_of1.
     + invc_value_typeof. invc_vtm. invc_ctm.
-      destruct n; eexists; right; left; eauto using tstep, mstep.
+      destruct n; eexists; right; right; left; eauto using tstep, mstep.
     + eexists. left. repeat eexists. intros Hfalse.
       specialize (Hmstep Hfalse). invc_mstep. eauto using tstep, mstep.
     + eexists. right. left. repeat eexists. intros He.
       specialize (Hmstep He). invc_mstep; eauto using tstep, mstep.
+    + eexists. right. right. left. repeat eexists. intros He.
+      specialize (Hmstep He). invc_mstep; eauto using tstep, mstep.
     + eexists. right. right. repeat eexists. eauto using tstep.
-  - eexists. right. left. eauto using tstep, mstep. 
-  - rewrite HeqGamma in *. unfold empty, Map.empty' in *. auto.
-  - destructIH IHtype_of1.
+  - repeat spec. eexists. right. right. left. eauto using tstep, mstep. 
+  - unfold empty, Map.empty' in *. auto.
+  - repeat spec. destructIH IHtype_of1.
     + invc_value_typeof. invc_vtm. invc_ctm.
       destructIH IHtype_of2; eexists.
-      * right. left. eauto using tstep, mstep.
+      * right. right. left. eauto using tstep, mstep.
       * left. repeat eexists. intros Hfalse.
         specialize (Hmstep Hfalse). invc_mstep. eauto using value, tstep, mstep.
       * right. left. repeat eexists. intros He.
+        specialize (Hmstep He). invc_mstep; eauto using value, tstep, mstep.
+      * right. right. left. repeat eexists. intros He.
         specialize (Hmstep He). invc_mstep; eauto using value, tstep, mstep.
       * right. right. repeat eexists. eauto using value, tstep.
     + eexists. left. repeat eexists. intros Hfalse.
       specialize (Hmstep Hfalse). invc_mstep. eauto using tstep, mstep.
     + eexists. right. left. repeat eexists. intros He.
       specialize (Hmstep He). invc_mstep; eauto using tstep, mstep.
+    + eexists. right. right. left. repeat eexists. intros He.
+      specialize (Hmstep He). invc_mstep; eauto using tstep, mstep.
     + eexists. right. right. repeat eexists. eauto using tstep.
-  - destructIH IHtype_of; eexists; right; left; eauto using tstep, mstep.
-  - destructIH IHtype_of; eexists; right; left; eauto using tstep, mstep.
-  - destructIH IHtype_of; eexists; right; left; eauto using tstep, mstep.
-  - destructIH IHtype_of; eexists.
-    + right. left. eauto using tstep, mstep.
+  - repeat spec.
+    destructIH IHtype_of; eexists; right; right; left; eauto using tstep, mstep.
+  - rewrite <- empty_eq_safe_empty in *. repeat spec.
+    destructIH IHtype_of; eexists; right; right; left; eauto using tstep, mstep.
+  - repeat spec. 
+    destructIH IHtype_of; eexists; right; right; left; eauto using tstep, mstep.
+  - repeat spec. destructIH IHtype_of; eexists.
+    + right. right. left. eauto using tstep, mstep.
     + left. repeat eexists. intros Hfalse.
       specialize (Hmstep Hfalse). invc_mstep. eauto using tstep, mstep.
     + right. left. repeat eexists. intros He.
       specialize (Hmstep He). invc_mstep; eauto using tstep, mstep.
+    + right. right. left. repeat eexists. intros He.
+      specialize (Hmstep He). invc_mstep; eauto using tstep, mstep.
     + right. right. repeat eexists. eauto using tstep.
-  - destructIH IHtype_of; eexists.
-    + right. left. eauto using tstep, mstep.
+  - repeat spec. destructIH IHtype_of; eexists.
+    + right. right. left. eauto using tstep, mstep.
     + left. repeat eexists. intros Hfalse.
       specialize (Hmstep Hfalse). invc_mstep. eauto using tstep, mstep.
     + right. left. repeat eexists. intros He.
       specialize (Hmstep He). invc_mstep; eauto using tstep, mstep.
+    + right. right. left. repeat eexists. intros He.
+      specialize (Hmstep He). invc_mstep; eauto using tstep, mstep.
     + right. right. repeat eexists. eauto using tstep.
-  - destructIH IHtype_of; eexists.
-    + right. left. eauto using tstep, mstep.
+  - repeat spec. destructIH IHtype_of; eexists.
+    + right. right. left. eauto using tstep, mstep.
     + left. repeat eexists. intros Hfalse.
       specialize (Hmstep Hfalse). invc_mstep. eauto using tstep, mstep.
     + right. left. repeat eexists. intros He.
       specialize (Hmstep He). invc_mstep; eauto using tstep, mstep.
+    + right. right. left. repeat eexists. intros He.
+      specialize (Hmstep He). invc_mstep; eauto using tstep, mstep.
     + right. right. repeat eexists. eauto using tstep.
-  - destructIH IHtype_of.
+  - repeat spec. destructIH IHtype_of.
     + invc_value_typeof. invc_vtm. invc_ctm.
-      eexists. right. left. eauto using tstep, mstep.
+      eexists. right. right. left. eauto using tstep, mstep.
     + eexists. left. repeat eexists. intros Hfalse.
       specialize (Hmstep Hfalse). invc_mstep. eauto using tstep, mstep.
     + eexists. right. left. repeat eexists. intros He.
       specialize (Hmstep He). invc_mstep; eauto using tstep, mstep.
+    + eexists. right. right. left. repeat eexists. intros He.
+      specialize (Hmstep He). invc_mstep; eauto using tstep, mstep.
     + eexists. right. right. repeat eexists. eauto using tstep.
-  - destructIH IHtype_of.
+  - repeat spec. destructIH IHtype_of.
     + invc_value_typeof. invc_vtm. invc_ctm.
-      eexists. right. left. eauto using tstep, mstep.
+      eexists. right. right. left. eauto using tstep, mstep.
     + eexists. left. repeat eexists. intros Hfalse.
       specialize (Hmstep Hfalse). invc_mstep. eauto using tstep, mstep.
     + eexists. right. left. repeat eexists. intros He.
       specialize (Hmstep He). invc_mstep; eauto using tstep, mstep.
+    + eexists. right. right. left. repeat eexists. intros He.
+      specialize (Hmstep He). invc_mstep; eauto using tstep, mstep.
     + eexists. right. right. repeat eexists. eauto using tstep.
-  - destructIH IHtype_of1.
+  - repeat spec. destructIH IHtype_of1.
     + invc_value_typeof. invc_vtm. invc_ctm.
       destructIH IHtype_of2; eexists.
-      * right. left. eauto using tstep, mstep.
+      * right. right. left. eauto using tstep, mstep.
       * left. repeat eexists. intros Hfalse.
         specialize (Hmstep Hfalse). invc_mstep. eauto using value, tstep, mstep.
       * right. left. repeat eexists. intros He.
+        specialize (Hmstep He). invc_mstep; eauto using value, tstep, mstep.
+      * right. right. left. repeat eexists. intros He.
         specialize (Hmstep He). invc_mstep; eauto using value, tstep, mstep.
       * right. right. repeat eexists. eauto using value, tstep.
     + eexists. left. repeat eexists. intros Hfalse.
       specialize (Hmstep Hfalse). invc_mstep. eauto using tstep, mstep.
     + eexists. right. left. repeat eexists. intros He.
       specialize (Hmstep He). invc_mstep; eauto using tstep, mstep.
+    + eexists. right. right. left. repeat eexists. intros He.
+      specialize (Hmstep He). invc_mstep; eauto using tstep, mstep.
     + eexists. right. right. repeat eexists. eauto using tstep.
-  - destructIH IHtype_of1.
+  - repeat spec. destructIH IHtype_of1.
     + invc_value_typeof. invc_vtm. invc_ctm.
-      eexists. left. eauto using tstep, mstep.
+      eexists. left. repeat eexists. eauto using tstep, mstep.
     + eexists. left. repeat eexists. intros Hfalse.
       specialize (Hmstep Hfalse). invc_mstep. eauto using tstep, mstep.
     + eexists. right. left. repeat eexists. intros He.
       specialize (Hmstep He). invc_mstep; eauto using tstep, mstep.
-    + eexists. right. right. repeat eexists. eauto using tstep.
-  - destructIH IHtype_of; eexists.
-    + right. left. eauto using tstep, mstep.
-    + left. repeat eexists. intros Hfalse.
-      specialize (Hmstep Hfalse). invc_mstep. eauto using tstep, mstep.
-    + right. left. repeat eexists. intros He.
+    + eexists. right. right. left. repeat eexists. intros He.
       specialize (Hmstep He). invc_mstep; eauto using tstep, mstep.
-    + right. right. repeat eexists. eauto using tstep.
-  - destructIH IHtype_of; eexists;
-    right; right; exists 0; eexists; eauto using tstep.
+    + eexists. right. right. repeat eexists. eauto using tstep.
+  - spec. spec. spec. specialize (IHtype_of (WR_ad ad)).
+    assert (WR_ad ad <> WR_self) by (intros F; invc F). spec.
+    repeat spec. destructIH IHtype_of.
+    + eexists. right. right. left. repeat eexists. eauto using tstep, mstep.
+    + eexists. left. repeat eexists. intros Hfalse.
+      specialize (Hmstep Hfalse). invc_mstep. eauto using tstep, mstep.
+    + eexists. right. left. repeat eexists. intros He.
+      specialize (Hmstep He). invc_mstep; eauto using tstep, mstep.
+    + eexists. right. right. left. repeat eexists. intros He.
+      specialize (Hmstep He). invc_mstep; eauto using tstep, mstep.
+    + eexists. right. right. repeat eexists. eauto using tstep.
+  - invc_typeof. invc_vtm. invc_ctm.
+    eexists. right. right. left. repeat eexists. intro.
+    eauto using tstep, mstep.
+  - eexists. right. left. repeat eexists. intro.
+    eauto using tstep, mstep.
+  - eexists. right. right. right. repeat eexists.
+    eauto using tstep.
 Qed.
 
 (*
@@ -442,7 +553,7 @@ Theorem limited_progress : forall m1 t1,
   (value t1
     \/ (exists m2 t2,      m1 \ t1 ==[e_none       ]==> m2 \ t2)
     \/ (exists m2 t2 ad T, m1 \ t1 ==[e_alloc ad T ]==> m2 \ t2)
-    \/ (exists m2 t2 ad t, m1 \ t1 ==[e_insert ad t]==> m2 \ t2)
+    \/ (exists m2 t2 ad t, m1 \ t1 ==[e_init ad t]==> m2 \ t2)
     \/ (exists m2 t2 ad t, m1 \ t1 ==[e_read ad t  ]==> m2 \ t2)
     \/ (exists m2 t2 ad t, m1 \ t1 ==[e_write ad t ]==> m2 \ t2)
     \/ (exists m2 t2 ad t, m1[ad].X = false ->
@@ -465,17 +576,17 @@ Proof.
   - pick_alloc. repeat eexists. eauto using tstep, mstep.
   - repeat spec.
     destruct_IH; try solve [solve_inductive_progress_case].
-    pick_insert.
+    pick_init.
     invc_value_typeof;
     repeat eexists; eauto using tstep, mstep, value.
   - repeat spec.
     destruct_IH; try solve [solve_inductive_progress_case].
-    pick_insert.
+    pick_init.
     invc_value_typeof;
     repeat eexists; eauto using tstep, mstep, value.
   - repeat spec.
     destruct_IH; try solve [solve_inductive_progress_case].
-    pick_insert.
+    pick_init.
     invc_value_typeof;
     repeat eexists; eauto using tstep, mstep, value.
   - repeat spec.
