SyntacticProperties.v
@@ -1,15 +1,22 @@
 From Elo Require Export NoRef.
 From Elo Require Export NoInit.
 From Elo Require Export NoCR.
+From Elo Require Export NoReacq.
+
 From Elo Require Export HasVar.
 From Elo Require Export NoWRef.
 
+From Elo Require Export Keywords.
 From Elo Require Export ValidTerm.
+From Elo Require Export ConsistentWaits.
+
 From Elo Require Export InheritanceNoInit.
 From Elo Require Export InheritanceNoCR.
 From Elo Require Export OneInit.
 From Elo Require Export OneCR.
 From Elo Require Export NoUninitRefs.
 From Elo Require Export UniqueInits.
-From Elo Require Export UniqueCRs.
+From Elo Require Export Waiting.
+From Elo Require Export Holding.
+From Elo Require Export UniqueHolding.
 
