UniqueHolding.v
@@ -1,0 +1,383 @@
+From Elo Require Import Core.
+
+From Elo Require Import NoCR.
+From Elo Require Import NoReacq.
+From Elo Require Import ValidTerm.
+From Elo Require Import ConsistentWaits.
+From Elo Require Import OneCR.
+From Elo Require Import Waiting.
+From Elo Require Import Holding.
+
+(* ------------------------------------------------------------------------- *)
+(* unique-holding                                                            *)
+(* ------------------------------------------------------------------------- *)
+
+Definition unique_holding (m : mem) (ths : threads) := forall ad,
+  (m[ad].X = false -> forall_threads ths (not_holding ad)) /\
+  (m[ad].X = true  -> forone_thread  ths (holding ad) (not_holding ad)).
+
+(* lemmas ------------------------------------------------------------------ *)
+
+Corollary hg_or_nhg_from_uhg : forall ad m ths tid,
+  unique_holding m ths ->
+  holding ad ths[tid] \/ not_holding ad ths[tid].
+Proof.
+  intros * Huhg. specialize (Huhg ad) as [? Htrue].
+  destruct (m[ad].X); spec; eauto.
+  specialize Htrue as [tid' [? ?]].
+  nat_eq_dec tid' tid; auto.
+Qed.
+
+Corollary nocr_or_onecr_from_uhg : forall ad m ths tid,
+  unique_holding m ths ->
+  no_cr ad ths[tid] \/ one_cr ad ths[tid].
+Proof.
+  intros * Huhg. specialize (Huhg ad) as [Hfalse Htrue].
+  destruct (m[ad].X); spec.
+  - specialize Htrue as [tid' [[? ?] Hnhg]].
+    nat_eq_dec tid' tid; auto.
+    specialize (Hnhg tid). spec. destruct Hnhg as [? | [? ?]]; eauto.
+  - specialize (Hfalse tid). destruct Hfalse as [? | [? ?]]; eauto.
+Qed.
+
+Corollary uhg_hg_contradiction : forall ad m ths tid1 tid2,
+  unique_holding m ths ->
+  (* --- *)
+  tid1 <> tid2 ->
+  holding ad ths[tid1] ->
+  holding ad ths[tid2] ->
+  False.
+Proof.
+  intros * Huhg **. specialize (Huhg ad) as [? Htrue].
+  destruct (m[ad].X); spec;
+  eauto using hg_contradiction.
+  specialize Htrue as [tid [? ?]].
+  nat_eq_dec tid1 tid; nat_eq_dec tid2 tid;
+  eauto using hg_contradiction.
+Qed.
+
+Corollary uhg_hg_equality : forall ad m ths tid1 tid2,
+  unique_holding m ths ->
+  (* --- *)
+  holding ad ths[tid1] ->
+  holding ad ths[tid2] ->
+  tid1 = tid2.
+Proof.
+  intros. nat_eq_dec tid1 tid2; trivial. exfalso.
+  eauto using uhg_hg_contradiction.
+Qed.
+
+Lemma locked_from_holding : forall m ths tid ad,
+  unique_holding m ths ->
+  (* --- *)
+  holding ad ths[tid] ->
+  m[ad].X = true.
+Proof.
+  intros * Huhg ?.
+  destruct (m[ad].X) eqn:Heq; trivial.
+  specialize (Huhg ad) as [? _]. spec.
+  exfalso. eauto using hg_contradiction.
+Qed.
+
+Lemma locked_from_rel : forall m ths tid t ad,
+  forall_threads ths (valid_term m) ->
+  unique_holding m ths     ->
+  (* --- *)
+  ths[tid] --[e_rel ad]--> t ->
+  m[ad].X = true.
+Proof.
+  intros * ? Huhg ?.
+  destruct (m[ad].X) eqn:Heq; trivial.
+  specialize (Huhg ad) as [Hnholding _]. spec.
+  exfalso. specialize (Hnholding tid) as [? | [? ?]];
+  eauto using nocr_rel_contradiction, wg_effect_contradiction.
+Qed.
+
+Lemma locked_from_wrel : forall m ths tid t ad,
+  forall_threads ths (valid_term m) ->
+  forall_threads ths (consistent_waits WR_none) ->
+  unique_holding m ths     ->
+  (* --- *)
+  ths[tid] --[e_wrel ad]--> t ->
+  m[ad].X = true.
+Proof.
+  intros * ? ? Huhg ?.
+  destruct (m[ad].X) eqn:Heq; trivial.
+  specialize (Huhg ad) as [Hnholding _]. spec.
+  exfalso. specialize (Hnholding tid) as [? | [? ?]];
+  eauto using nocr_wrel_contradiction, wg_effect_contradiction.
+Qed.
+
+(* preservation lemmas ----------------------------------------------------- *)
+
+Lemma uhg_mem_region : forall m ths ad R,
+  unique_holding m ths ->
+  unique_holding m[ad.R <- R] ths.
+Proof.
+  intros * H. intros ad'. specialize (H ad').
+  repeat omicron; upsilon; destruct H; trivial;
+  split; repeat intro; repeat omicron; upsilon; spec; eauto.
+Qed.
+
+(* preservation ------------------------------------------------------------ *)
+
+Local Lemma uhg_preservation_none : forall m ths tid t,
+  forall_threads ths (valid_term m) ->
+  (* --- *)
+  tid < #ths ->
+  unique_holding m ths ->
+  ths[tid] --[e_none]--> t ->
+  unique_holding m ths[tid <- t].
+Proof.
+  intros until 1.
+  intros ? Huhg ? ad. specialize (Huhg ad) as [Hfall Hfone].
+  split; intros; spec.
+  - intros ?. omicron; eauto using nhg_preservation_none.
+  - specialize Hfone as [tid' [? ?]]. exists tid'. split; intros; omicron;
+    eauto using nhg_preservation_none, hg_preservation_none.
+Qed.
+
+Local Lemma uhg_preservation_alloc : forall m ths tid t T R,
+  tid < #ths ->
+  unique_holding m ths ->
+  ths[tid] --[e_alloc (#m) T]--> t ->
+  unique_holding (m +++ new_cell T R) ths[tid <- t].
+Proof.
+  intros *.
+  intros ? Huhg ? ad. specialize (Huhg ad) as [Hfall Hfone].
+  split; intros; upsilon; spec.
+  - intros ?. omicron; eauto using nhg_preservation_alloc.
+  - specialize Hfone as [tid' [? ?]]. exists tid'.
+    split; intros; omicron;
+    eauto using nhg_preservation_alloc, hg_preservation_alloc.
+Qed.
+
+Local Lemma uhg_preservation_init : forall m ths tid t ad' t',
+  forall_threads ths (valid_term m) ->
+  (* --- *)
+  tid < #ths ->
+  unique_holding m ths ->
+  ths[tid] --[e_init ad' t']--> t ->
+  unique_holding m[ad'.t <- t'] ths[tid <- t].
+Proof.
+  intros until 1.
+  intros ? Huhg ? ad. specialize (Huhg ad) as [Hfall Hfone].
+  assert (ad' < #m) by eauto using vtm_init_address.
+  split; intros; omicron; upsilon; spec; solve
+    [ intro; omicron; eauto using nhg_preservation_init
+    | specialize Hfone as [tid' [? ?]]; exists tid';
+      split; intros; omicron;
+      eauto using nhg_preservation_init, hg_preservation_init
+    ].
+Qed.
+
+Local Lemma uhg_preservation_read : forall m ths tid t ad te,
+  value te ->
+  valid_term m te ->
+  (* --- *)
+  tid < #ths ->
+  unique_holding m ths ->
+  ths[tid] --[e_read ad te]--> t ->
+  unique_holding m ths[tid <- t].
+Proof.
+  intros until 2.
+  intros ? Huhg ? ad'. specialize (Huhg ad') as [Hfall Hfone].
+  split; intros; upsilon; spec.
+  - intros ?. omicron; eauto using nhg_preservation_read.
+  - specialize Hfone as [tid' [? ?]]. exists tid'.
+    split; intros; omicron;
+    eauto using nhg_preservation_read, hg_preservation_read.
+Qed.
+
+Local Lemma uhg_preservation_write : forall m ths tid t ad te,
+  forall_threads ths (valid_term m) ->
+  (* --- *)
+  tid < #ths ->
+  unique_holding m ths ->
+  ths[tid] --[e_write ad te]--> t ->
+  unique_holding m[ad.t <- te] ths[tid <- t].
+Proof.
+  intros until 1.
+  intros ? Huhg ? ad'. specialize (Huhg ad') as [Hfall Hfone].
+  assert (ad < #m) by eauto using vtm_write_address.
+  split; intros; repeat omicron; spec; upsilon;
+  eauto using nhg_unit, nhg_preservation_write;
+  specialize Hfone as [tid' [? ?]]; exists tid'; split; intros;
+  omicron; eauto using nhg_preservation_write, hg_preservation_write.
+Qed.
+
+Local Lemma uhg_preservation_acq : forall m ths tid ad t te,
+  value te ->
+  valid_term m te ->
+  forall_threads ths (valid_term m) ->
+  forall_threads ths (consistent_waits WR_none) ->
+  (* --- *)
+  m[ad].X = false ->
+  tid < #ths ->
+  unique_holding m ths ->
+  ths[tid] --[e_acq ad te]--> t ->
+  unique_holding m[ad.X <- true] ths[tid <- t].
+Proof.
+  intros until 5.
+  intros ? Huhg ? ad'. specialize (Huhg ad') as [Hfall Hfone].
+  assert (ad < #m) by eauto using vtm_acq_address.
+  split; intros; repeat omicron; spec; upsilon;
+  eauto using nhg_unit, nhg_preservation_acq.
+  - exists tid. sigma. split.
+    + split.
+      * specialize (Hfall tid) as [? | [? ?]].
+        ** eauto using nocrs_from_value, nocr_to_onecr.
+        ** exfalso. eauto using wg_effect_contradiction.
+      * specialize (Hfall tid) as [? | [? ?]].
+        ** eauto using noreacq_from_value, noreacq_preservation_acq,
+            noreacq_from_nocr.
+        ** exfalso. eauto using wg_effect_contradiction.
+    + intros. sigma. eauto.
+  - specialize Hfone as [tid' [? ?]]. exists tid'. split.
+    + omicron; eauto using hg_preservation_acq.
+    + intros. omicron; eauto using nhg_preservation_acq.
+Qed.
+
+Local Lemma uhg_preservation_rel : forall m ths tid ad t,
+  forall_threads ths (valid_term m) ->
+  (* --- *)
+  tid < #ths ->
+  unique_holding m ths ->
+  ths[tid] --[e_rel ad]--> t ->
+  unique_holding m[ad.X <- false] ths[tid <- t].
+Proof.
+  intros until 1.
+  intros ? Huhg ? ad'. destruct (Huhg ad') as [Hfall Hfone].
+  assert (Had : m[ad].X = true) by eauto using locked_from_rel.
+  split; intros; try intros tid'; repeat omicron; spec; upsilon;
+  auto; eauto using nhg_preservation_rel;
+  specialize Hfone as [tid'' [Hholding Hnholding]].
+  - destruct Hholding. nat_eq_dec tid'' tid'.
+    + left. eauto using onecr_to_nocr.
+    + specialize (Hnholding tid'). spec. destruct Hnholding as [? | [? ?]];
+      exfalso; eauto using nocr_rel_contradiction, wg_effect_contradiction.
+  - nat_eq_dec tid'' tid'; auto.
+    specialize (Hnholding tid). spec. destruct Hnholding as [? | [? ?]];
+    exfalso; eauto using nocr_rel_contradiction, wg_effect_contradiction.
+  - exists tid''. nat_eq_dec tid'' tid; sigma;
+    split; eauto using hg_preservation_rel; intros.
+    + sigma. auto.
+    + omicron; eauto using nhg_preservation_rel.
+Qed.
+
+Local Lemma uhg_preservation_wacq : forall m ths tid t ad,
+  forall_threads ths (valid_term m) ->
+  forall_threads ths (consistent_waits WR_none) ->
+  (* --- *)
+  m[ad].X = false ->
+  tid < #ths ->
+  unique_holding m ths ->
+  ths[tid] --[e_wacq ad]--> t ->
+  unique_holding m[ad.X <- true] ths[tid <- t].
+Proof.
+  intros until 3.
+  intros ? Huhg ? ad'. specialize (Huhg ad') as [Hfall Hfone].
+  assert (ad < #m) by eauto using vtm_wacq_address.
+  split; intros; repeat omicron; spec; upsilon;
+  eauto using nhg_unit, nhg_preservation_wacq.
+  - exists tid. sigma. split.
+    + split.
+      * specialize (Hfall tid) as [? | [? ?]].
+        ** exfalso. eauto using noreacq_from_nocr, noreacq_wacq_contradiction.
+        ** eauto using onecr_preservation_wacq.
+      * specialize (Hfall tid) as [? | [? ?]].
+        ** eauto using nocr_preservation_wacq, cw_preservation_wacq,
+            noreacq_from_nocr.
+        ** eauto using wg_to_noreacq.
+    + intros. sigma. eauto.
+  - specialize Hfone as [tid' [? ?]]. exists tid'. split.
+    + omicron; eauto using hg_preservation_wacq.
+    + intros. omicron; eauto using nhg_preservation_wacq.
+Qed.
+
+Local Lemma uhg_preservation_wrel : forall m ths tid ad t,
+  forall_threads ths (valid_term m) ->
+  forall_threads ths (consistent_waits WR_none) ->
+  (* --- *)
+  tid < #ths ->
+  unique_holding m ths ->
+  ths[tid] --[e_wrel ad]--> t ->
+  unique_holding m[ad.X <- false] ths[tid <- t].
+Proof.
+  intros until 2.
+  intros ? Huhg ? ad'. destruct (Huhg ad') as [Hfall Hfone].
+  assert (Had : m[ad].X = true) by eauto using locked_from_wrel.
+  split; intros; try intros tid'; repeat omicron; spec; upsilon;
+  auto; eauto using nhg_preservation_wrel;
+  specialize Hfone as [tid'' [Hhg Hnhg]].
+  - destruct Hhg. nat_eq_dec tid'' tid'.
+    + right. split; eauto using onecr_preservation_wrel, noreacq_to_wg.
+    + specialize (Hnhg tid'). spec. exfalso. destruct Hnhg as [? | [? ?]];
+      eauto using nocr_wrel_contradiction, wg_effect_contradiction.
+  - nat_eq_dec tid'' tid'; auto.
+    destruct Hhg. specialize (Hnhg tid). spec. exfalso.
+    destruct Hnhg as [? | [? ?]];
+    eauto using nocr_wrel_contradiction, wg_effect_contradiction.
+  - exists tid''. nat_eq_dec tid'' tid; sigma;
+    split; eauto using hg_preservation_wrel; intros.
+    + sigma. auto.
+    + omicron; eauto using nhg_preservation_wrel.
+Qed.
+
+Local Ltac eapply_in_tstep tt :=
+  match goal with Htstep : _ --[_]--> _ |- _ => eapply tt in Htstep as ? end.
+
+Local Lemma uhg_preservation_spawn : forall m ths tid t t',
+  forall_threads ths (valid_term m) ->
+  (* --- *)
+  tid < #ths ->
+  unique_holding m ths ->
+  ths[tid] --[e_spawn t']--> t ->
+  unique_holding m (ths[tid <- t] +++ t').
+Proof.
+  intros until 1.
+  intros ? Huhg ? ad'. destruct (Huhg ad') as [Hfall Hfone].
+  split; intros; spec.
+  - intro. omicron;
+    eauto using nhg_preservation_spawn, nhg_unit.
+    left. eauto using nocr_spawn_term.
+  - specialize Hfone as [tid' [Hholding Hnholding]]. exists tid'. split.
+    + omicron; eauto.
+      * eauto using hg_preservation_spawn.
+      * destruct Hholding. invc_onecr.
+    + intros. omicron; eauto using nhg_preservation_spawn, nhg_unit.
+      left. eauto using nocr_spawn_term.
+Qed.
+
+Theorem uhg_preservation_cstep : forall m1 m2 ths1 ths2 tid e,
+  forall_memory  m1 value                ->
+  forall_program m1 ths1 (valid_term m1) ->
+  forall_program m1 ths1 (consistent_waits WR_none) ->
+  (* --- *)
+  unique_holding m1 ths1 ->
+  m1 \ ths1 ~~[tid, e]~~> m2 \ ths2 ->
+  unique_holding m2 ths2.
+Proof.
+  intros * ? [? ?] [? ?] **. invc_cstep; try invc_mstep.
+  - eauto using uhg_preservation_none.
+  - sigma. upsilon. eauto using uhg_preservation_alloc.
+  - eauto using uhg_preservation_init.
+  - eauto using uhg_preservation_read.
+  - eauto using uhg_preservation_write.
+  - eauto using uhg_preservation_acq.
+  - eauto using uhg_preservation_rel.
+  - eauto using uhg_preservation_wacq.
+  - eauto using uhg_preservation_wrel.
+  - eauto using uhg_preservation_spawn.
+Qed.
+
+Theorem uhg_preservation_base : forall t,
+  no_crs t ->
+  (* --- *)
+  unique_holding nil (base t).
+Proof.
+  unfold base. intros ** ?. split; intros Hnil.
+  - intro. left. omicron; auto using no_cr.
+  - simpl in Hnil. destruct ad; upsilon; auto.
+Qed.
+
