Waiting.v
@@ -1,0 +1,338 @@
+From Elo Require Import Core.
+
+From Elo Require Import NoCR.
+From Elo Require Import NoReacq.
+From Elo Require Import ValidTerm.
+From Elo Require Import OneCR.
+
+(* ------------------------------------------------------------------------- *)
+(* waiting                                                                   *)
+(* ------------------------------------------------------------------------- *)
+
+Inductive waiting (ad : addr) : tm -> Prop :=
+  | wg_plus1  : forall t1 t2,    waiting  ad t1 ->
+                                 no_reacq ad t2 ->
+                                 waiting ad <{t1 + t2               }>
+  | wg_plus2  : forall t1 t2,    value t1       ->
+                                 waiting  ad t2 ->
+                                 waiting  ad <{t1 + t2              }>
+  | wg_monus1 : forall t1 t2,    waiting  ad t1 ->
+                                 no_reacq ad t2 ->
+                                 waiting  ad <{t1 - t2              }>
+  | wg_monus2 : forall t1 t2,    value t1       ->
+                                 waiting  ad t2 ->
+                                 waiting  ad <{t1 - t2              }>
+  | wg_seq    : forall t1 t2,    waiting  ad t1 ->
+                                 waiting  ad <{t1; t2               }>
+  | wg_if     : forall t1 t2 t3, waiting  ad t1 ->
+                                 waiting  ad (tm_if t1 t2 t3) 
+  | wg_call1  : forall t1 t2,    waiting  ad t1 ->
+                                 no_reacq ad t2 ->
+                                 waiting  ad <{call t1 t2           }>
+  | wg_call2  : forall t1 t2,    value t1       ->
+                                 waiting  ad t2 ->
+                                 waiting  ad <{call t1 t2           }>
+  | wg_init   : forall ad' t T,  waiting  ad t  ->
+                                 waiting  ad <{init ad' t : T       }>
+  | wg_load   : forall t,        waiting  ad t  ->
+                                 waiting  ad <{*t                   }>
+  | wg_asg1   : forall t1 t2,    waiting  ad t1 ->
+                                 no_reacq ad t2 ->
+                                 waiting  ad <{t1 := t2             }>
+  | wg_asg2   : forall t1 t2,    value t1       ->
+                                 waiting  ad t2 ->
+                                 waiting  ad <{t1 := t2             }>
+  | wg_acq    : forall t1 x t2,  waiting  ad t1 ->
+                                 waiting  ad <{acq t1 x t2          }>
+  | wg_cr     : forall ad' t,    waiting  ad t  ->
+                                 waiting  ad <{cr ad' t             }>
+  | wg_wait   : forall t,        waiting  ad t  ->
+                                 waiting  ad <{wait t               }>
+  | wg_reacq  :                  waiting  ad <{reacq ad             }>
+  .
+
+(* inversion --------------------------------------------------------------- *)
+
+Local Ltac _wg tt :=
+  match goal with
+  | H : waiting _   <{unit                  }> |- _ => invc H
+  | H : waiting _   <{nat _                 }> |- _ => invc H
+  | H : waiting _   <{_ + _                 }> |- _ => tt H
+  | H : waiting _   <{_ - _                 }> |- _ => tt H
+  | H : waiting _   <{_; _                  }> |- _ => tt H
+  | H : waiting _   <{if _ then _ else _ end}> |- _ => tt H
+  | H : waiting _   <{while _ do _ end      }> |- _ => invc H
+  | H : waiting _   <{var _                 }> |- _ => invc H
+  | H : waiting _   <{fn _ _ _              }> |- _ => invc H
+  | H : waiting _   <{call _ _              }> |- _ => tt H
+  | H : waiting _   <{&_ : _                }> |- _ => invc H
+  | H : waiting _   <{new _ : _             }> |- _ => invc H
+  | H : waiting _   <{init _ _ : _          }> |- _ => tt H
+  | H : waiting _   <{* _                   }> |- _ => tt H
+  | H : waiting _   <{_ := _                }> |- _ => tt H
+  | H : waiting _   <{acq _ _ _             }> |- _ => tt H
+  | H : waiting _   <{cr _ _                }> |- _ => tt H
+  | H : waiting _   <{wait _                }> |- _ => tt H
+  | H : waiting ?ad <{reacq ?ad             }> |- _ => clear H
+  | H : waiting _   <{reacq _               }> |- _ => tt H
+  | H : waiting _   <{spawn _               }> |- _ => invc H
+  end.
+
+Ltac inv_wg  := _wg inv.
+Ltac invc_wg := _wg invc.
+
+(* preservation lemmas ----------------------------------------------------- *)
+
+Lemma wg_subst : forall ad m x tx t,
+  valid_term m t ->
+  (* --- *)
+  no_reacq   ad tx -> 
+  waiting ad t  ->
+  waiting ad <{[x := tx] t}>.
+Proof.
+  intros. induction t; invc_vtm; invc_wg;
+  simpl; repeat destruct _str_eq_dec;
+  auto using value_subst, noreacq_subst, waiting.
+Qed.
+
+(* lemmas ------------------------------------------------------------------ *)
+
+Lemma _value_does_not_wait : forall ad t,
+  value t ->
+  waiting ad t ->
+  False.
+Proof.
+  intros * Hval ?. invc Hval; invc_wg.
+Qed.
+
+Ltac value_does_not_wait :=
+  match goal with _ : value ?t, _ : waiting _ ?t |- _ =>
+    solve [exfalso; eauto using _value_does_not_wait]
+  end.
+
+Lemma wg_ad_bound : forall ad m t,
+  valid_term m t ->
+  (* --- *)
+  waiting ad t ->
+  ad < #m.
+Proof.
+  intros. induction t; invc_vtm; invc_wg; auto.
+Qed.
+
+Lemma noreacq_wg_contradiction : forall ad t,
+  no_reacq ad t ->
+  waiting  ad t ->
+  False.
+Proof.
+  intros. induction t; invc_noreacq; invc_wg; auto.
+Qed.
+
+Corollary noreacqs_wg_contradiction : forall ad t,
+  no_reacqs t ->
+  waiting ad t ->
+  False.
+Proof.
+  unfold no_reacqs. eauto using noreacq_wg_contradiction.
+Qed.
+
+Lemma noreacq_to_wg : forall t1 t2 ad,
+  no_reacq ad t1 ->
+  t1 --[e_wrel ad]--> t2 ->
+  waiting ad t2.
+Proof.
+  intros. ind_tstep; invc_noreacq;
+  auto using noreacq_subst, no_reacq, waiting.
+Qed.
+
+Lemma wg_to_noreacq : forall m t1 t2 ad,
+  valid_term m t1 ->
+  (* --- *)
+  waiting ad t1 ->
+  t1 --[e_wacq ad]--> t2 ->
+  no_reacq ad t2.
+Proof.
+  intros. ind_tstep; invc_vtm; invc_wg; try value_does_not_step;
+  eauto using noreacq_from_value, no_reacq;
+  exfalso; eauto using noreacq_wacq_contradiction.
+Qed.
+
+Lemma wg_to_wg_contradiction : forall t1 t2 ad,
+  waiting ad t1 ->
+  t1 --[e_wrel ad]--> t2 ->
+  waiting ad t2 ->
+  False.
+Proof.
+  intros. ind_tstep; repeat invc_wg; auto;
+  try value_does_not_step; try value_does_not_wait;
+  eauto using wg_subst, noreacq_to_wg, noreacq_wg_contradiction.
+Qed.
+
+Lemma wg_effect_contradiction : forall m t1 t2 ad e,
+  valid_term m t1 ->
+  (* --- *)
+  waiting ad t1 ->
+  t1 --[e]--> t2   ->
+  e <> e_wacq ad   ->
+  False.
+Proof.
+  intros * ? ? ? Hneq. apply Hneq.
+  ind_tstep; invc_vtm; repeat invc_wg; auto;
+  value_does_not_step || value_does_not_wait.
+Qed.
+
+(* preservation ------------------------------------------------------------ *)
+
+Local Ltac solve_wg_preservation L :=
+  intros; ind_tstep; try invc_vtm; repeat invc_wg;
+  try value_does_not_step; try value_does_not_wait;
+  eauto using L, wg_subst, waiting;
+  exfalso; eauto using noreacqs_from_value, noreacqs_wg_contradiction.
+
+Lemma wg_preservation_none : forall ad m t1 t2,
+  valid_term m t1 ->
+  (* --- *)
+  waiting ad t1 ->
+  t1 --[e_none]--> t2 ->
+  waiting ad t2.
+Proof. solve_wg_preservation noreacq_preservation_none. Qed.
+
+Lemma wg_preservation_alloc : forall ad t1 t2 ad' T',
+  waiting ad t1 ->
+  t1 --[e_alloc ad' T']--> t2 ->
+  waiting ad t2.
+Proof. solve_wg_preservation noreacq_preservation_alloc. Qed.
+
+Lemma wg_preservation_init : forall ad m t1 t2 ad' t',
+  valid_term m t1 ->
+  (* --- *)
+  waiting ad t1 ->
+  t1 --[e_init ad' t']--> t2 ->
+  waiting ad t2.
+Proof. solve_wg_preservation noreacq_preservation_init. Qed.
+
+Lemma wg_preservation_read : forall ad t1 t2 ad' t',
+  no_reacq ad t' ->
+  (* --- *)
+  waiting ad t1 ->
+  t1 --[e_read ad' t']--> t2 ->
+  waiting ad t2.
+Proof. solve_wg_preservation noreacq_preservation_read. Qed.
+
+Lemma wg_preservation_write : forall ad m t1 t2 ad' t',
+  valid_term m t1 ->
+  (* --- *)
+  waiting ad t1 ->
+  t1 --[e_write ad' t']--> t2 ->
+  waiting ad t2.
+Proof. solve_wg_preservation noreacq_preservation_write. Qed.
+
+Lemma wg_preservation_acq : forall ad t1 t2 ad' t',
+  no_reacq ad t' ->
+  (* --- *)
+  waiting ad t1 ->
+  t1 --[e_acq ad' t']--> t2 ->
+  waiting ad t2.
+Proof. solve_wg_preservation noreacq_preservation_acq. Qed.
+
+Lemma wg_preservation_rel : forall ad t1 t2 ad',
+  waiting ad t1 ->
+  t1 --[e_rel ad']--> t2 ->
+  waiting ad t2.
+Proof. solve_wg_preservation noreacq_preservation_rel. Qed.
+
+Lemma wg_preservation_wacq : forall ad t1 t2 ad',
+  ad <> ad' ->
+  waiting ad t1 ->
+  t1 --[e_wacq ad']--> t2 ->
+  waiting ad t2.
+Proof. solve_wg_preservation noreacq_preservation_wacq. Qed.
+
+Lemma wg_preservation_wrel : forall ad t1 t2 ad',
+  waiting ad t1 ->
+  t1 --[e_wrel ad']--> t2 ->
+  waiting ad t2.
+Proof. solve_wg_preservation noreacq_preservation_wrel. Qed.
+
+Lemma wg_preservation_spawn : forall ad m t1 t2 t',
+  valid_term m t1 ->
+  (* --- *)
+  waiting ad t1 ->
+  t1 --[e_spawn t']--> t2 ->
+  waiting ad t2.
+Proof. solve_wg_preservation noreacq_preservation_spawn. Qed.
+
+(* inheritance ------------------------------------------------------------- *)
+
+(*
+Local Ltac solve_wg_inheritance L :=
+  intros; ind_tstep; repeat invc_vtm; try invc_wg; auto;
+  eauto using L, noreacq_from_value, waiting; exfalso;
+  match goal with H : waiting ?ad ?t |- _ =>
+    apply (noreacq_wg_contradiction ad t);
+    eauto using noreacq_from_value, noreacq_subst, no_reacq
+  end.
+
+Lemma wg_inheritance_none : forall ad m t1 t2,
+  valid_term m t1 ->
+  (* --- *)
+  waiting ad t2 ->
+  t1 --[e_none]--> t2 ->
+  waiting ad t1.
+Proof. solve_wg_inheritance noreacq_inheritance_none. Qed.
+
+Lemma wg_inheritance_alloc : forall ad t1 t2 ad' T',
+  waiting ad t2 ->
+  t1 --[e_alloc ad' T']--> t2 ->
+  waiting ad t1.
+Proof. solve_wg_inheritance noreacq_inheritance_alloc. Qed.
+
+Lemma wg_inheritance_init : forall ad m t1 t2 ad' t',
+  valid_term m t1 ->
+  (* --- *)
+  waiting ad t2 ->
+  t1 --[e_init ad' t']--> t2 ->
+  waiting ad t1.
+Proof. solve_wg_inheritance noreacq_inheritance_init. Qed.
+
+Lemma wg_inheritance_read : forall ad t1 t2 ad' t',
+  no_reacqs t' ->
+  (* --- *)
+  waiting ad t2 ->
+  t1 --[e_read ad' t']--> t2 ->
+  waiting ad t1.
+Proof. solve_wg_inheritance noreacq_inheritance_read. Qed.
+
+Lemma wg_inheritance_write : forall ad m t1 t2 ad' t',
+  valid_term m t1 ->
+  (* --- *)
+  waiting ad t2 ->
+  t1 --[e_write ad' t']--> t2 ->
+  waiting ad t1.
+Proof. solve_wg_inheritance noreacq_inheritance_write. Qed.
+
+Lemma wg_inheritance_acq : forall ad m t1 t2 ad' t',
+  valid_term m t1 ->
+  no_reacqs t' ->
+  (* --- *)
+  ad <> ad' ->
+  waiting ad t2 ->
+  t1 --[e_acq ad' t']--> t2 ->
+  waiting ad t1.
+Proof. solve_wg_inheritance noreacq_inheritance_acq. Qed.
+
+Lemma wg_inheritance_rel : forall ad t1 t2 ad',
+  ad <> ad' ->
+  waiting ad t2 ->
+  t1 --[e_rel ad']--> t2 ->
+  waiting ad t1.
+Proof. solve_wg_inheritance noreacq_inheritance_rel. Qed.
+
+Lemma wg_inheritance_spawn : forall ad m t1 t2 t',
+  valid_term m t1 ->
+  (* --- *)
+  waiting ad t2 ->
+  t1 --[e_spawn t']--> t2 ->
+  waiting ad t1.
+Proof. solve_wg_inheritance noreacq_inheritance_spawn. Qed.
+*)
+
